\subsection{Senkrechte (E-Feld) Polarisation (H-Feld parallel)}
\input{Figures/SchraegerUebergang_senk_Polarisation.tex}

\[ \boxed{\texttt{mit } Z_{F0} = 120\pi \approx 377\si{\ohm}} \]
\begin{align*}
    Z_{Fn}                & = Z_{F0}\cdot\frac{1}{\sqrt{\varepsilon_{rn}}}            \\
    \frac{Z_{F1}}{Z_{F2}} & = \frac{\sqrt{\varepsilon_{r2}}}{\sqrt{\varepsilon_{r1}}}
\end{align*}
\[ n: \texttt{Brechungsindex} \quad ; \quad \theta_h = \theta_r\]
\begin{align*}
    \frac{\sin\theta_t}{\sin\theta_h} & = \frac{\lambda_2}{\lambda_1}= \frac{\beta_1}{\beta_2}= \frac{n_1}{n_2} \\
    \sin\theta_t                      & = \sqrt{\frac{\varepsilon_{r1}}{\varepsilon_{r2}}}\cdot \sin\theta_h
\end{align*}

\begin{itemize}
    \item magnetischer/elektrischer Reflexionsfaktor $[1]$
    \item magnetischer Transmissionsfaktor $[1]$
    \item elektrischer Transmissionsfaktor $[1]$
\end{itemize}
\begin{align*}
    r_s    & =  r_{es} = r_{ms} =                                                                                                                                            \\
           & = \frac{Z_{F2} \cdot \cos \theta_h-Z_{F1} \cdot \cos \theta_t}{Z_{F2} \cdot \cos \theta_h+Z_{F1} \cdot \cos \theta_t}                                           \\
           & = \frac{\cos\theta_h-\sqrt{^{\varepsilon_{r2}}/_{\varepsilon_{r1}}-\sin^2\theta_h}}{\cos\theta_h+\sqrt{^{\varepsilon_{r2}}/_{\varepsilon_{r1}}-\sin^2\theta_h}} \\
    t_{ms} & = Z_{F1} \cdot \frac{2 \cdot \cos \theta_h}{Z_{F2} \cdot \cos \theta_h+Z_{F1} \cdot \cos \theta_t}                                                              \\
           & = (1 - r_s) \cdot \dfrac{\cos \theta_h}{\cos \theta_t}                                                                                                          \\
           & = \frac{Z_{F1}}{Z_{F2}}\cdot t_{es}                                                                                                                             \\
    t_{es} & = Z_{F2} \cdot \frac{2 \cdot \cos \theta_h}{Z_{F2} \cdot \cos \theta_h+Z_{F1} \cdot \cos \theta_t}                                                              \\
           & = 1+r_s
\end{align*}

\begin{align*}
    E_r & = r_s \cdot E_h    \\
    E_t & = t_{es} \cdot E_h \\
    H_r & = r_s \cdot H_h    \\
    H_t & = t_{ms} \cdot H_h \\
    E_t & = H_t\cdot Z_{F2}  \\
    E_h & = H_h\cdot Z_{F1}
\end{align*}

\subsection{Parallel (E-Feld) Polarisation (H-Feld senkrecht)}
\input{Figures/SchraegerUebergang_para_Polaristion.tex}

\[ \boxed{\texttt{mit } Z_{F0} = 120\pi \approx 377\si{\ohm}} \]
\begin{align*}
    Z_{Fn}                & = Z_{F0}\cdot\frac{1}{\sqrt{\varepsilon_{rn}}}            \\
    \frac{Z_{F1}}{Z_{F2}} & = \frac{\sqrt{\varepsilon_{r2}}}{\sqrt{\varepsilon_{r1}}}
\end{align*}
\[ n: \texttt{Brechungsindex} \quad ; \quad \theta_h = \theta_r\]
\begin{align*}
    \frac{\sin\theta_t}{\sin\theta_h} & = \frac{\lambda_2}{\lambda_1}= \frac{\beta_1}{\beta_2}= \frac{n_1}{n_2} \\
    \sin\theta_t                      & = \sqrt{\frac{\varepsilon_{r1}}{\varepsilon_{r2}}}\cdot\sin\theta_h
\end{align*}

\begin{itemize}
    \item magnetischer/elektrischer Reflexionsfaktor $[1]$
    \item magnetischer Transmissionsfaktor $[1]$
    \item elektrischer Transmissionsfaktor $[1]$
\end{itemize}
\begin{align*}
    r_p    & =  r_{ep} = r_{mp} =                                                                                                                                                                                                        \\
           & = \frac{Z_{F2} \cdot \cos \theta_t-Z_{F1} \cdot \cos \theta_h}{Z_{F2} \cdot \cos \theta_t+Z_{F1} \cdot \cos \theta_h} =                                                                                                     \\
           & = \frac{\varepsilon_{r2}\cos\theta_h-\sqrt{\varepsilon_{r2}\varepsilon_{r1}-{\varepsilon_{r1}}^2\sin^2\theta_h}}{\varepsilon_{r2}\cos\theta_h+\sqrt{{\varepsilon_{r2}\varepsilon_{r1}-{\varepsilon_{r1}}^2\sin^2\theta_h}}} \\
    t_{mp} & = Z_{F1} \cdot \frac{2 \cdot \cos \theta_h}{Z_{F1} \cdot \cos \theta_h+Z_{F2} \cdot \cos \theta_t}                                                                                                                          \\
           & = 1+r_p                                                                                                                                                                                                                     \\
    t_{ep} & = Z_{F2} \cdot \frac{2 \cdot \cos \theta_h}{Z_{F1} \cdot \cos \theta_h+Z_{F2} \cdot \cos \theta_t}                                                                                                                          \\
           & = (1-r_p) \cdot \dfrac{\cos \theta_h}{\cos \theta_t}                                                                                                                                                                        \\
           & = \frac{Z_{F2}}{Z_{F1}}\cdot t_{mp}
\end{align*}

\begin{align*}
    E_r & = r_p\cdot E_h    \\
    E_t & = t_{ep}\cdot E_h \\
    H_r & = r_p\cdot H_h    \\
    H_t & = t_{mp}\cdot H_h \\
    E_t & = H_t\cdot Z_{F2} \\
    E_h & = H_h\cdot Z_{F1}
\end{align*}
